lean/disaster-recovery/DisasterRecovery/Shared/Capabilities.lean
@@ -2,7 +2,9 @@ import Std
 
 namespace DisasterRecovery.Shared
 
-structure Capabilities (σ Node Message : Type) where
-  send : Message -> Node -> ST σ Unit
+abbrev Effect (Node Message : Type) := StateM (List (Node × Message))
+
+structure Capabilities (Node Message : Type) where
+  send : Message -> Node -> Effect Node Message Unit
 
 end DisasterRecovery.Shared
